theories/coneris/examples/hash/con_hash_impl2.v
@@ -33,40 +33,36 @@ Section con_hash_impl2.
     )%I.
   Definition hash_tape α ns γ2 γ_tape :=
     (hash_tape1 α ns γ2 γ_tape (* ∗ [∗ list] n∈ns, hash_set_frag n γ5 *))%I.
-  Definition hash_tape_auth m γ2 γ3 :=
-    (hash_tape_auth1 m γ2 γ3
-    )%I.
 
   Definition hash_frag k v γ1 γ2 γ4:=
     (hv_frag (L:=Hhv) k v γ4 ∗
      hash_frag1 k v γ1 γ2)%I.
 
-  Definition con_hash_inv N f l hm (P:gmap nat nat -> gmap val (list nat) -> iProp Σ) {HP: ∀ m m', Timeless (P m m')} R {HR:∀ m, Timeless (R m)} γ1 γ2 γ_tape γ4 γ5 γ_lock:=
-    con_hash_inv1 N f l hm (λ m m', P m m')%I (λ m, hv_auth (L:=Hhv) m γ4 ∗ ([∗ map] v∈m, (v ↪[γ5] ())) ∗ R m)%I γ1 γ2  γ_tape γ_lock.
+  Definition con_hash_inv N f l hm R {HR:∀ m, Timeless (R m)} γ1 γ2 γ_tape γ4 γ5 γ_lock:=
+    con_hash_inv1 N f l hm (λ m, hv_auth (L:=Hhv) m γ4 ∗ ([∗ map] v∈m, (v ↪[γ5] ())) ∗ R m)%I γ1 γ2  γ_tape γ_lock.
 
-  Lemma hash_tape_presample N f l hm P {HP: ∀ m m', Timeless (P m m')} R {HR:∀ m, Timeless (R m)} m γ_hv γ_set γ_hv' γ γ_set' γ_lock α ns s (ε εO:nonnegreal) E:
-  ↑(N.@"rand")⊆E ->
+  Lemma hash_tape_presample N f l hm R {HR: ∀ m, Timeless (R m )} γ_hv γ_set γ_hv' γ γ_set' γ_lock α ns s (ε εO:nonnegreal) E:
+  ↑(N)⊆E ->
   (INR s + εO * (val_size + 1 - INR s) <= ε * (val_size + 1))%R ->
-  con_hash_inv N f l hm P R γ_hv γ_set γ γ_hv' γ_set' γ_lock -∗
-    hash_tape_auth m γ_set γ -∗ hash_tape α ns γ_set γ-∗ ↯ ε -∗
+  con_hash_inv N f l hm R γ_hv γ_set γ γ_hv' γ_set' γ_lock -∗
+    hash_tape α ns γ_set γ-∗ ↯ ε -∗
     hash_set s γ_set γ_set'-∗
-    state_update E E (∃ (n:fin(S val_size)),
+    state_update E E (∃ (n:fin(S val_size)), 
           (  hash_set (s+1)%nat γ_set γ_set' ∗ ↯ εO
           )∗
-          hash_tape_auth (<[α:=ns++[fin_to_nat n]]>m) γ_set γ ∗
           hash_tape α (ns++[fin_to_nat n]) γ_set γ ∗ hash_set_frag (fin_to_nat n) γ_set γ_set'
       ).
   Proof.
-    rewrite /hash_tape_auth/hash_tape/hash_set/hash_set_frag.
-    iIntros (Hsubset Hineq) "#Hinv Htauth Ht Herr (%s' & <- & Hset & Hset')".
+    rewrite /hash_tape/hash_set/hash_set_frag.
+    iIntros (Hsubset Hineq) "#Hinv Ht Herr (%s' & <- & Hset & Hset')".
     iPoseProof (hash_set_valid with "Hset") as "%Hbound".
-    iMod (con_hash_interface1.hash_tape_presample _ _ _ _ _ _ _ _ _ _ _ _ _ _ s' _ 1%NNR with "[//][$][$][$][$]") as "Hcont".
+    iMod (con_hash_interface1.hash_tape_presample _ _ _ _ _ _ _ _ _ _ _ _ s' _ 1%NNR with "[//][$][$][$]") as "Hcont".
     { done. }
     { intros.
       by apply Nat.lt_succ_r, Hbound.
     }
     { simpl. erewrite Rmult_1_l. done. }
-    iDestruct ("Hcont" ) as "(%&[(%&?)|(%&?)]&?&$&$)".
+    iDestruct ("Hcont" ) as "(%&[(%&?)|(%&?)]&?&$)".
     { by iDestruct (ec_contradict with "[$]") as "%". }
     iMod (ghost_map_insert with "[$]") as "[Hset' Hs']".
     { apply not_elem_of_dom_1. by rewrite dom_gset_to_gmap. }
@@ -78,30 +74,10 @@ Section con_hash_impl2.
     - iApply (hash_set_duplicate); last done. set_solver.
   Qed.
 
-  Lemma con_hash_presample  N f l hm P {HP: ∀ m m', Timeless (P m m')} R {HR:∀ m, Timeless (R m)} γ_hv γ_set γ_tape γ_hv' γ_set' γ_lock Q
-    E  :
-    ↑(N.@"hash") ⊆ E ->
-    con_hash_inv N f l hm P R γ_hv γ_set γ_tape γ_hv' γ_set' γ_lock -∗
-    (∀ m m', P m m'  -∗
-             hash_tape_auth m' γ_set γ_tape -∗
-             state_update (E∖↑(N.@"hash")) (E∖↑(N.@"hash"))
-             (∃ m'', P m m'' ∗ hash_tape_auth m'' γ_set γ_tape ∗ Q m m' m'')
-    ) -∗
-    state_update E E (
-        ∃ m m' m'', Q m m' m''
-      ) .
-  Proof.
-    iIntros (Hsubset) "#Hinv Hvs".
-    iMod (con_hash_presample1 with "[//][-]"); first done; last done.
-    rewrite /hash_tape_auth.
-    iIntros (??) "??".
-    by iMod ("Hvs" with "[$][$]") as "(%&$&$)".
-  Qed.
-
-  Lemma con_hash_init N P {HP: ∀ m m', Timeless (P m m')} R {HR:∀ m, Timeless (R m)}:
-    {{{ P ∅ ∅ ∗ R ∅}}}
+  Lemma con_hash_init N R {HR:∀ m, Timeless (R m)}:
+    {{{ R ∅}}}
       init_hash #()
-      {{{ (f:val), RET f; ∃ l hm γ1 γ2 γ3 γ4 γ5 γ_lock, con_hash_inv N f l hm P R γ1 γ2 γ3 γ4 γ5 γ_lock ∗
+      {{{ (f:val), RET f; ∃ l hm γ1 γ2 γ3 γ4 γ5 γ_lock, con_hash_inv N f l hm R γ1 γ2 γ3 γ4 γ5 γ_lock ∗
                                                   hash_set 0%nat γ2 γ5
       }}}.
   Proof.
@@ -115,36 +91,28 @@ Section con_hash_impl2.
     - iIntros (f)"(%l &%hm&%γ1&%γ2&%γ3&%γ_lock&#H1&H2)".
       iApply "HΦ". rewrite /con_hash_inv/hash_set.
       by iFrame "H1 H2 H'".
-    - iDestruct "HP" as "[$$]". by iFrame.
+    - by iFrame.
   Qed.
 
-  Lemma con_hash_alloc_tape N f l hm P {HP: ∀ m m', Timeless (P m m')} R {HR:∀ m, Timeless (R m)} γ1 γ2 γ3 γ4 γ5 γ_lock Q:
-  {{{ con_hash_inv N f l hm P R γ1 γ2 γ3 γ4 γ5 γ_lock ∗
-      (∀ m m' α, P m m' -∗ ⌜α∉dom m'⌝ -∗ |={⊤∖↑N.@"hash"}=> P m (<[α:=[]]>m') ∗ Q α)
+  Lemma con_hash_alloc_tape N f l hm R {HR:∀ m, Timeless (R m)} γ1 γ2 γ3 γ4 γ5 γ_lock:
+  {{{ con_hash_inv N f l hm R γ1 γ2 γ3 γ4 γ5 γ_lock 
   }}}
       allocate_tape #()
-      {{{ (α: val), RET α; hash_tape α [] γ2 γ3 ∗ Q α }}}.
+      {{{ (α: val), RET α; hash_tape α [] γ2 γ3 }}}.
   Proof.
-    iIntros (Φ) "[#Hinv Hvs] HΦ".
+    iIntros (Φ) "#Hinv HΦ".
     rewrite /allocate_tape.
-    wp_apply (con_hash_alloc_tape1 with "[Hvs $Hinv]").
-    - iIntros (???) "?%".
-      iMod ("Hvs" with "[$][//]") as "[$ H]".
-      iFrame.
-      iApply "H".
-    - rewrite /hash_tape.
-      iIntros (?) "[??]".
-      iApply "HΦ". iFrame.
+    by wp_apply (con_hash_alloc_tape1 with "[$Hinv]").
   Qed.
 
-  Lemma con_hash_spec  N f l hm P {HP: ∀ m m', Timeless (P m m')} R {HR: ∀ m, Timeless (R m )} γ1 γ2 γ3 γ4 γ5 γ_lock Q1 Q2 α (v:nat):
-  {{{ con_hash_inv N f l hm P R γ1 γ2 γ3 γ4 γ5 γ_lock ∗ 
-      ( ∀ m m', R m -∗ P m m' -∗ hash_tape_auth m' γ2 γ3 -∗ hash_auth m γ1 γ2 γ4 γ5-∗ state_update (⊤∖↑N.@"hash") (⊤∖↑N.@"hash")
+  Lemma con_hash_spec N f l hm R {HR: ∀ m, Timeless (R m )} γ1 γ2 γ3 γ4 γ5 γ_lock Q1 Q2 α (v:nat):
+  {{{ con_hash_inv N f l hm R γ1 γ2 γ3 γ4 γ5 γ_lock ∗ 
+      ( ∀ m, R m -∗  hash_auth m γ1 γ2 γ4 γ5-∗ state_update (⊤) (⊤)
              match m!!v with
-             | Some res => R m ∗ P m m' ∗ hash_tape_auth m' γ2 γ3 ∗ hash_auth m γ1 γ2 γ4 γ5∗ Q1 res
-             | None => ∃ n ns, hash_tape α (n::ns) γ2 γ3 ∗ P m (<[α:=n::ns]> m') ∗ hash_tape_auth (<[α:=n::ns]> m') γ2 γ3 ∗
-                              (∀ m'', P m m'' -∗ hash_tape α (ns) γ2 γ3 -∗ ⌜m''!!α=Some (n::ns)⌝
-                                      ={⊤∖↑N.@"hash"}=∗ R (<[v:=n]> m) ∗ P (<[v:=n]> m) (<[α:=ns]> m'') ∗
+             | Some res => R m ∗ hash_auth m γ1 γ2 γ4 γ5∗ Q1 res
+             | None => ∃ n ns, hash_tape α (n::ns) γ2 γ3 ∗ 
+                              (hash_tape α (ns) γ2 γ3 
+                                      ={⊤}=∗ R (<[v:=n]> m) ∗ 
                                       hash_auth (<[v:=n]> m) γ1 γ2 γ4 γ5∗ Q2 n ns)
              end                                        
       )
@@ -157,25 +125,25 @@ Section con_hash_impl2.
   Proof.
     iIntros (Φ) "(#Hinv  & Hvs) HΦ".
     rewrite /hash_tape/hash_set_frag.
-    iApply (con_hash_spec1 _ _ _ _ _ _ _ _ _ _ Q1 Q2 with "[$Hinv Hvs]").
-    - iIntros (??) "(Hhv & Hfrag & HR) HP Htauth Hauth1".
+    iApply (con_hash_spec1 _ _ _ _ _ _ _ _ _ Q1 Q2 with "[$Hinv Hvs]").
+    - iIntros (?) "(Hhv & Hfrag & HR) Hauth1".
       rewrite /hash_auth.
       rewrite /hash_set_frag.
-      iMod ("Hvs" with "[$][$][$][Hauth1 $Hhv Hfrag]") as "Hcont".
+      iMod ("Hvs" with "[$][Hauth1 $Hhv Hfrag]") as "Hcont".
       { rewrite big_sepM_sep. iFrame "Hfrag". iSplit; first done.
         rewrite big_sepM_forall. iIntros.
         iDestruct (con_hash_interface1.hash_auth_duplicate with "[$]") as "#?"; first done.
         by iApply hash_frag_in_hash_set.
       }
       case_match.
-      + iDestruct "Hcont" as "($&$&$&($&?&H)&$)".
+      + iDestruct "Hcont" as "($&($&?&H)&$)".
         iFrame.
         rewrite big_sepM_sep.
         by iDestruct "H" as "[??]".
-      + iDestruct "Hcont" as "(%&%&?&?&?&Hcont)".
+      + iDestruct "Hcont" as "(%&%&?&Hcont)".
         iModIntro.
         iFrame. iIntros.
-        iMod ("Hcont" with "[$][$][//]") as "(?&?&(?&?&H)&?)".
+        iMod ("Hcont" with "[$]") as "(?&(?&?&H)&?)".
         iFrame.
         rewrite big_sepM_sep.
         iDestruct "H" as "[??]". by iFrame.
@@ -194,11 +162,9 @@ Section con_hash_impl2.
       hash_tape2:=hash_tape;
       hash_frag2:=hash_frag;
       hash_auth2:=hash_auth;
-      hash_tape_auth2 := hash_tape_auth;
       hash_set2:=hash_set;
       hash_set_frag2:=hash_set_frag;
       con_hash_interface2.hash_tape_presample := hash_tape_presample;
-      con_hash_presample2 := con_hash_presample;
       con_hash_init2 := con_hash_init;
       con_hash_alloc_tape2 := con_hash_alloc_tape;
       con_hash_spec2:=con_hash_spec
@@ -255,10 +221,6 @@ Section con_hash_impl2.
     rewrite /hash_set_frag.
     iModIntro. rewrite big_sepM_sep.
     by iFrame.
-  Qed.
-  Next Obligation.
-    iIntros.
-    iApply (con_hash_interface1.hash_tape_auth_frag_agree with "[$][$]").
   Qed.
   Next Obligation.
     iIntros (????) "?".
