theories/coneris/examples/hash/con_hash_interface0.v
@@ -20,25 +20,21 @@ Class con_hash0 `{!conerisGS Σ} (val_size:nat):= Con_Hash0
   hash_lock_gname:Type;
   
   (** * Predicates *)
-  con_hash_inv0 (N:namespace) (f l hm: val) (P:gmap nat nat -> gmap val (list nat) -> iProp Σ) {HP: ∀ m m', Timeless (P m m')}
-    (R:gmap nat nat -> iProp Σ) {HR: ∀ m, Timeless (R m )} (γ:hash_tape_gname) (γ_lock:hash_lock_gname): iProp Σ;
+  con_hash_inv0 (N:namespace) (f l hm: val) (R:gmap nat nat -> iProp Σ) {HR: ∀ m, Timeless (R m )} (γ:hash_tape_gname) (γ_lock:hash_lock_gname): iProp Σ;
   (* concrete_seq_hash {L:seq_hashG Σ} (f:val) (m:gmap nat nat) : iProp Σ;  *)
   hash_tape0 (α:val) (ns:list nat) (γ:hash_tape_gname): iProp Σ;
-  hash_tape_auth0 (m:gmap val (list nat)) (γ:hash_tape_gname) :iProp Σ;
   (* hash_auth0 (m:gmap nat nat) (γ2:hash_view_gname) : iProp Σ; *)
   (* hash_frag0 (v res:nat) (γ:hash_view_gname): iProp Σ; *)
   
   (** * General properties of the predicates *)
   #[global] hash_tape_timeless α ns γ::
     Timeless (hash_tape0 α ns γ); 
-  #[global] hash_tape_auth_timeless m γ::
-    Timeless (hash_tape_auth0 m γ);
   (* #[global] hash_map_timeless m γ :: *)
   (*   Timeless (hash_auth0 m γ); *)
   (* #[global] hash_frag_timeless v res γ :: *)
   (*   Timeless (hash_frag0 v res γ); *)
-  #[global] con_hash_inv_persistent N f l hm P {HP: ∀ m m', Timeless (P m m')} R {HR: ∀ m, Timeless (R m )} γ_tape γ_lock ::
-    Persistent (con_hash_inv0 N f l hm P R γ_tape γ_lock); 
+  #[global] con_hash_inv_persistent N f l hm R {HR: ∀ m, Timeless (R m )} γ_tape γ_lock ::
+    Persistent (con_hash_inv0 N f l hm R γ_tape γ_lock); 
   (* #[global] hash_frag_persistent v res γ :: *)
   (*   Persistent (hash_frag0 v res γ); *)
   
@@ -48,19 +44,16 @@ Class con_hash0 `{!conerisGS Σ} (val_size:nat):= Con_Hash0
     hash_tape0 α ns γ-∗ hash_tape0 α ns' γ-∗ False;
   (* hash_tape_auth_exclusive m m' γ: *)
   (*   hash_tape_auth0 m γ -∗ hash_tape_auth0 m' γ -∗ False; *)
-  hash_tape_auth_frag_agree m α ns γ:
-    hash_tape_auth0 m γ  -∗ hash_tape0 α ns γ -∗ ⌜m!!α=Some ns⌝;
   (* hash_tape_auth_alloc m α γ: *)
   (*   m!!α=None -> hash_tape_auth0 m γ ==∗ hash_tape_auth0 (<[α:=[]]> m) γ ∗ hash_tape0 α [] γ; *)
-  hash_tape_presample N m γ γ_lock f l hm P {HP: ∀ m m', Timeless (P m m')} R {HR: ∀ m, Timeless (R m )} α ns ε ε2 E:
-  ↑(N.@"rand")⊆E ->
+  hash_tape_presample N γ γ_lock f l hm R {HR: ∀ m, Timeless (R m )} α ns ε ε2 E:
+  ↑(N)⊆E ->
     (∀ x : fin (S val_size), (0 <= ε2 x)%R)->
     (SeriesC (λ n : fin (S val_size), 1 / S val_size * ε2 n) <= ε)%R ->
-    con_hash_inv0 N f l hm P R γ γ_lock -∗
-    hash_tape_auth0 m γ -∗ hash_tape0 α ns γ -∗ ↯ ε -∗
+    con_hash_inv0 N f l hm R γ γ_lock -∗
+    hash_tape0 α ns γ -∗ ↯ ε -∗
     state_update E E (∃ n, 
           ↯ (ε2 n) ∗
-          hash_tape_auth0 (<[α:=ns++[fin_to_nat n]]>m) γ ∗
           hash_tape0 α (ns++[fin_to_nat n]) γ); 
   (* hash_auth_exclusive m m' γ: *)
   (*   hash_auth0 m γ -∗ hash_auth0 m' γ -∗ False; *)
@@ -72,39 +65,37 @@ Class con_hash0 `{!conerisGS Σ} (val_size:nat):= Con_Hash0
   (*   m!!k=None -> hash_auth0 m γ ==∗ (hash_auth0 (<[k:=v]> m) γ ∗ hash_frag0 k v γ); *)
                       
 
-  con_hash_presample0 N f l hm P {HP: ∀ m m', Timeless (P m m')} R {HR: ∀ m, Timeless (R m )} γ γ_lock Q
-    E  :
-    ↑(N.@"hash") ⊆ E ->
-    con_hash_inv0 N f l hm P R γ γ_lock -∗
-    (∀ m m', P m m'  -∗
-             hash_tape_auth0 m' γ -∗
-             state_update (E∖↑(N.@"hash")) (E∖↑(N.@"hash"))
-             (∃ m'', P m m'' ∗ hash_tape_auth0 m'' γ ∗ Q m m' m'')
-    ) -∗
-    state_update E E (
-        ∃ m m' m'', Q m m' m''
-      ); 
+  (* con_hash_presample0 N f l hm P {HP: ∀ m m', Timeless (P m m')} R {HR: ∀ m, Timeless (R m )} γ γ_lock Q *)
+  (*   E  : *)
+  (*   ↑(N.@"hash") ⊆ E -> *)
+  (*   con_hash_inv0 N f l hm P R γ γ_lock -∗ *)
+  (*   (∀ m m', P m m'  -∗ *)
+  (*            hash_tape_auth0 m' γ -∗ *)
+  (*            state_update (E∖↑(N.@"hash")) (E∖↑(N.@"hash")) *)
+  (*            (∃ m'', P m m'' ∗ hash_tape_auth0 m'' γ ∗ Q m m' m'') *)
+  (*   ) -∗ *)
+  (*   state_update E E ( *)
+  (*       ∃ m m' m'', Q m m' m'' *)
+  (*     );  *)
 
-  con_hash_init0 N P {HP: ∀ m m', Timeless (P m m')} R {HR: ∀ m, Timeless (R m )} :
-    {{{ P ∅ ∅ ∗ R ∅}}}
+  con_hash_init0 N R {HR: ∀ m, Timeless (R m )} :
+    {{{ R ∅}}}
       init_hash0 #()
-      {{{ (f:val), RET f; ∃ l hm γ_tape γ_lock, con_hash_inv0 N f l hm P R γ_tape γ_lock }}}; 
+      {{{ (f:val), RET f; ∃ l hm γ_tape γ_lock, con_hash_inv0 N f l hm R γ_tape γ_lock }}}; 
 
-  con_hash_alloc_tape0 N f l hm P {HP: ∀ m m', Timeless (P m m')} R {HR: ∀ m, Timeless (R m )} γ_tape γ_lock Q:
-  {{{ con_hash_inv0 N f l hm P R γ_tape γ_lock ∗
-      (∀ m m' α, P m m' -∗ ⌜α∉dom m'⌝ -∗ |={⊤∖↑N.@"hash"}=> P m (<[α:=[]]>m') ∗ Q α)
+  con_hash_alloc_tape0 N f l hm R {HR: ∀ m, Timeless (R m )} γ_tape γ_lock:
+  {{{ con_hash_inv0 N f l hm R γ_tape γ_lock
   }}}
       allocate_tape0 #()
-      {{{ (α: val), RET α; hash_tape0 α [] γ_tape ∗ Q α }}}; 
+      {{{ (α: val), RET α; hash_tape0 α [] γ_tape }}}; 
   
-  con_hash_spec0 N f l hm P {HP: ∀ m m', Timeless (P m m')} R {HR: ∀ m, Timeless (R m )} γ_tape γ_lock Q1 Q2 α (v:nat):
-  {{{ con_hash_inv0 N f l hm P R γ_tape γ_lock ∗ 
-      ( ∀ m m', R m -∗ P m m' -∗ hash_tape_auth0 m' γ_tape -∗ state_update (⊤∖↑N.@"hash") (⊤∖↑N.@"hash")
+  con_hash_spec0 N f l hm R {HR: ∀ m, Timeless (R m )} γ_tape γ_lock Q1 Q2 α (v:nat):
+  {{{ con_hash_inv0 N f l hm R γ_tape γ_lock ∗ 
+      ( ∀ m , R m -∗ state_update (⊤) (⊤)
              match m!!v with
-             | Some res => R m ∗ P m m' ∗ hash_tape_auth0 m' γ_tape ∗ Q1 res
-             | None => ∃ n ns, hash_tape0 α (n::ns) γ_tape ∗ P m (<[α:=n::ns]> m') ∗ hash_tape_auth0 (<[α:=n::ns]> m') γ_tape ∗
-                              (∀ m'', P m m'' -∗  hash_tape0 α (ns) γ_tape -∗ ⌜m''!!α=Some (n::ns)⌝
-                                      ={⊤∖↑N.@"hash"}=∗ R (<[v:=n]> m) ∗ P (<[v:=n]> m) (<[α:=ns]> m'') ∗ Q2 n ns)
+             | Some res => R m ∗ Q1 res
+             | None => ∃ n ns, hash_tape0 α (n::ns) γ_tape ∗ 
+                              (hash_tape0 α (ns) γ_tape ={⊤}=∗ R (<[v:=n]> m) ∗ Q2 n ns)
              end                                        
       )
   }}}
