theories/coneris/examples/hash/con_hash_interface1.v
@@ -20,10 +20,9 @@ Class con_hash1 `{!conerisGS Σ} (val_size:nat):= Con_Hash1
   hash_lock_gname:Type;
   
   (** * Predicates *)
-  con_hash_inv1 (N:namespace) (f l hm: val) (P:gmap nat nat -> gmap val (list nat) -> iProp Σ) {HP: ∀ m m', Timeless (P m m')}  (R:gmap nat nat -> iProp Σ) {HR: ∀ m, Timeless (R m )} (γ1:hash_view_gname) (γ2: hash_set_gname) (γ3:hash_tape_gname) (γ_lock:hash_lock_gname): iProp Σ;
+  con_hash_inv1 (N:namespace) (f l hm: val) (R:gmap nat nat -> iProp Σ) {HR: ∀ m, Timeless (R m )} (γ1:hash_view_gname) (γ2: hash_set_gname) (γ3:hash_tape_gname) (γ_lock:hash_lock_gname): iProp Σ;
   (* concrete_seq_hash {L:seq_hashG Σ} (f:val) (m:gmap nat nat) : iProp Σ;  *)
   hash_tape1 (α:val) (ns:list nat) (γ2: hash_set_gname) (γ3:hash_tape_gname): iProp Σ;
-  hash_tape_auth1 (m:gmap val (list nat)) (γ2 :hash_set_gname) (γ3:hash_tape_gname): iProp Σ;
   hash_auth1 (m:gmap nat nat) (γ:hash_view_gname) (γ2 : hash_set_gname): iProp Σ;
   hash_frag1 (v res:nat) (γ:hash_view_gname) (γ2 : hash_set_gname): iProp Σ;
   hash_set1 (s: gset nat) (γ2:hash_set_gname) : iProp Σ;
@@ -34,8 +33,6 @@ Class con_hash1 `{!conerisGS Σ} (val_size:nat):= Con_Hash1
   (*   Timeless (concrete_seq_hash (L:=L) f m); *)
   #[global] hash_tape_timeless α ns γ2 γ3::
     Timeless (hash_tape1 α ns γ2 γ3);
-  #[global] hash_tape_auth_timeless m γ2 γ3::
-    Timeless (hash_tape_auth1 m γ2 γ3);
   #[global] hash_auth_timeless m γ γ2::
     Timeless (hash_auth1 m γ γ2);
   #[global] hash_frag_timeless v res γ γ2::
@@ -44,8 +41,8 @@ Class con_hash1 `{!conerisGS Σ} (val_size:nat):= Con_Hash1
     Timeless (hash_set1 s γ2); 
   #[global] hash_set_frag_timeless s γ2 ::
     Timeless (hash_set_frag1 s γ2); 
-  #[global] con_hash_inv_persistent N f l hm γ1 γ2 γ3 P {HP: ∀ m m', Timeless (P m m')} R {HR: ∀ m, Timeless (R m )}  γ_lock ::
-    Persistent (con_hash_inv1 N f l hm P R γ1 γ2 γ3 γ_lock); 
+  #[global] con_hash_inv_persistent N f l hm γ1 γ2 γ3  R {HR: ∀ m, Timeless (R m )}  γ_lock ::
+    Persistent (con_hash_inv1 N f l hm R γ1 γ2 γ3 γ_lock); 
   #[global] hash_frag_persistent v res γ γ2::
     Persistent (hash_frag1 v res γ γ2);
   #[global] hash_set_frag_persistent s γ2 ::
@@ -70,8 +67,6 @@ Class con_hash1 `{!conerisGS Σ} (val_size:nat):= Con_Hash1
     m!!k=None -> hash_set_frag1 v γ2 -∗ hash_auth1 m γ1 γ2 ==∗ hash_auth1 (<[k:=v]> m ) γ1 γ2;
   (* hash_tape_auth_exclusive m m' γ2 γ3: *)
   (*   hash_tape_auth1 m γ2 γ3 -∗ hash_tape_auth1 m' γ2 γ3 -∗ False; *)
-  hash_tape_auth_frag_agree m α ns γ2 γ3:
-    hash_tape_auth1 m γ2 γ3 -∗ hash_tape1 α ns γ2 γ3 -∗ ⌜m!!α=Some ns⌝;
   (* hash_tape_auth_insert m α γ2 γ3: *)
   (*   m!!α=None -> hash_tape_auth1 m γ2 γ3 ==∗ hash_tape_auth1 (<[α:=[]]> m) γ2 γ3 ∗ hash_tape1 α [] γ2 γ3; *)
   (* hash_tape_auth_frag_update m α ns n γ2 γ3: *)
@@ -85,57 +80,42 @@ Class con_hash1 `{!conerisGS Σ} (val_size:nat):= Con_Hash1
       hash_tape1 α ns γ2 γ3-∗ hash_tape1 α ns' γ2 γ3 -∗ False;
 
   
-  hash_tape_presample N f l hm P {HP: ∀ m m', Timeless (P m m')} R {HR: ∀ m, Timeless (R m )}  m γ_hv γ_set γ γ_lock α ns s (bad : gset nat)(ε εI εO:nonnegreal) E:
-  ↑(N.@"rand")⊆E ->
+  hash_tape_presample N f l hm R {HR: ∀ m, Timeless (R m )} γ_hv γ_set γ γ_lock α ns s (bad : gset nat)(ε εI εO:nonnegreal) E:
+  ↑(N)⊆E ->
   (forall x : nat, x ∈ bad -> (x < S val_size)%nat) ->
   (εI * (size bad) + εO * (val_size + 1 - size bad) <= ε * (val_size + 1))%R ->
-  con_hash_inv1 N f l hm P R γ_hv γ_set γ γ_lock -∗
-    hash_tape_auth1 m γ_set γ -∗ hash_tape1 α ns γ_set γ -∗ ↯ ε -∗
+  con_hash_inv1 N f l hm R γ_hv γ_set γ γ_lock -∗
+    hash_tape1 α ns γ_set γ -∗ ↯ ε -∗
     hash_set1 s γ_set -∗
     state_update E E (∃ (n:fin(S val_size)), 
           ( (⌜fin_to_nat n ∈ bad⌝) ∗ ↯ εI  ∨
             (⌜fin_to_nat n ∉ bad⌝) ∗ ↯ εO
           )∗
           hash_set1 (s∪{[(fin_to_nat n)]}) γ_set ∗
-          hash_tape_auth1 (<[α:=ns++[fin_to_nat n]]>m) γ_set γ ∗
           hash_tape1 α (ns++[fin_to_nat n]) γ_set γ
-      ); 
-
-  con_hash_presample1  N f l hm P {HP: ∀ m m', Timeless (P m m')} R {HR: ∀ m, Timeless (R m )} γ_hv γ_set γ_tape γ_lock Q
-    E  :
-    ↑(N.@"hash") ⊆ E ->
-    con_hash_inv1 N f l hm P R γ_hv γ_set γ_tape γ_lock -∗
-    (∀ m m', P m m'  -∗
-             hash_tape_auth1 m' γ_set γ_tape -∗
-             state_update (E∖↑(N.@"hash")) (E∖↑(N.@"hash"))
-             (∃ m'', P m m'' ∗ hash_tape_auth1 m'' γ_set γ_tape ∗ Q m m' m'')
-    ) -∗
-    state_update E E (
-        ∃ m m' m'', Q m m' m''
-      ) ;
-
-  con_hash_init1 N P {HP: ∀ m m', Timeless (P m m')} R {HR: ∀ m, Timeless (R m )} :
-    {{{ P ∅ ∅ ∗ R ∅}}}
+      );
+  
+  con_hash_init1 N R {HR: ∀ m, Timeless (R m )} :
+    {{{ R ∅}}}
       init_hash1 #()
-      {{{ (f:val), RET f; ∃ l hm γ1 γ2 γ3 γ_lock, con_hash_inv1 N f l hm P R γ1 γ2 γ3 γ_lock ∗
+      {{{ (f:val), RET f; ∃ l hm γ1 γ2 γ3 γ_lock, con_hash_inv1 N f l hm R γ1 γ2 γ3 γ_lock ∗
                                                   hash_set1 ∅ γ2
       }}}; 
 
-  con_hash_alloc_tape1 N f l hm P {HP: ∀ m m', Timeless (P m m')} R {HR: ∀ m, Timeless (R m )} γ1 γ2 γ3 γ_lock Q:
-  {{{ con_hash_inv1 N f l hm P R γ1 γ2 γ3 γ_lock ∗
-      (∀ m m' α, P m m' -∗ ⌜α∉dom m'⌝ -∗ |={⊤∖↑N.@"hash"}=> P m (<[α:=[]]>m') ∗ Q α)
+  con_hash_alloc_tape1 N f l hm R {HR: ∀ m, Timeless (R m )} γ1 γ2 γ3 γ_lock:
+  {{{ con_hash_inv1 N f l hm R γ1 γ2 γ3 γ_lock 
   }}}
       allocate_tape1 #()
-      {{{ (α: val), RET α; hash_tape1 α [] γ2 γ3 ∗ Q α }}}; 
+      {{{ (α: val), RET α; hash_tape1 α [] γ2 γ3 }}}; 
 
-  con_hash_spec1 N f l hm P {HP: ∀ m m', Timeless (P m m')} R {HR: ∀ m, Timeless (R m )} γ1 γ2 γ3 γ_lock Q1 Q2 α (v:nat):
-  {{{ con_hash_inv1 N f l hm P R γ1 γ2 γ3 γ_lock ∗ 
-      ( ∀ m m', R m -∗ P m m' -∗ hash_tape_auth1 m' γ2 γ3 -∗ hash_auth1 m γ1 γ2 -∗ state_update (⊤∖↑N.@"hash") (⊤∖↑N.@"hash")
+  con_hash_spec1 N f l hm R {HR: ∀ m, Timeless (R m )} γ1 γ2 γ3 γ_lock Q1 Q2 α (v:nat):
+  {{{ con_hash_inv1 N f l hm R γ1 γ2 γ3 γ_lock ∗ 
+      ( ∀ m, R m -∗ hash_auth1 m γ1 γ2 -∗ state_update (⊤) (⊤)
              match m!!v with
-             | Some res => R m ∗ P m m' ∗ hash_auth1 m γ1 γ2 ∗ hash_tape_auth1 m' γ2 γ3 ∗ Q1 res
-             | None => ∃ n ns, hash_tape1 α (n::ns) γ2 γ3 ∗ P m (<[α:=n::ns]> m') ∗ hash_tape_auth1 (<[α:=n::ns]> m') γ2 γ3 ∗
-                              (∀ m'', P m m'' -∗ hash_tape1 α (ns) γ2 γ3 -∗ ⌜m''!!α=Some (n::ns)⌝
-                                      ={⊤∖↑N.@"hash"}=∗ R (<[v:=n]> m) ∗ P (<[v:=n]> m) (<[α:=ns]> m'') ∗
+             | Some res => R m ∗ hash_auth1 m γ1 γ2 ∗ Q1 res
+             | None => ∃ n ns, hash_tape1 α (n::ns) γ2 γ3 ∗ 
+                              (hash_tape1 α (ns) γ2 γ3 
+                                      ={⊤}=∗ R (<[v:=n]> m) ∗
                                       hash_auth1 (<[v:=n]> m) γ1 γ2  ∗ Q2 n ns)
              end                                        
       )
@@ -150,44 +130,10 @@ Class con_hash1 `{!conerisGS Σ} (val_size:nat):= Con_Hash1
 
 Section test.
   Context `{conerisGS Σ, !con_hash1 val_size}.
-
-  Lemma con_hash_presample_test N f l hm γ1 γ2 γ3 γlock  E (ε εI εO:nonnegreal) ns α s :
-    ↑N⊆E ->
-    (εI * (size s) + εO * (val_size + 1 - size s) <= ε * (val_size + 1))%R ->
-    con_hash_inv1 N f l hm (λ _ _, True) (λ _, True )γ1 γ2 γ3 γlock -∗
-    hash_tape1 α ns γ2 γ3 -∗
-    ↯ ε -∗
-    hash_set1 s γ2 -∗
-    state_update E E (∃ (n:fin (S val_size)),
-          hash_tape1 α (ns++[fin_to_nat n]) γ2 γ3 ∗
-          ( (⌜fin_to_nat n ∈ s⌝) ∗ ↯ εI ∨
-            (⌜fin_to_nat n ∉ s⌝) ∗ ↯ εO
-          ) ∗
-          hash_set1 (s∪{[(fin_to_nat n)]}) γ2
-      ).
-  Proof.
-    iIntros (Hsubset Hineq) "#Hinv Ht Herr Hs".
-    iDestruct (hash_set_valid with "[$]") as "%Hbound".
-    iMod (con_hash_presample1 _ _ _ _ _ _ _ _ _ _
-            (λ m m' m'', (∃ n : fin (S val_size), hash_tape1 α (ns ++ [fin_to_nat n]) γ2 γ3 ∗
-                                                    (⌜fin_to_nat n ∈ s⌝ ∗ ↯ εI ∨ ⌜fin_to_nat n ∉ s⌝ ∗ ↯ εO) ∗
-                                                    hash_set1 (s ∪ {[fin_to_nat n]}) γ2 ))%I with "[//][-]") as "Hcont".
-    - by apply nclose_subseteq'.
-    - iIntros (_ ?) "_ Hauth".
-      iMod (hash_tape_presample _ _ _ _ _ _ _ _ _ _ _ _ _ s with "[//][$][$][$][$]") as "(%&?&?&?&?)".
-      + apply subseteq_difference_r; last by apply nclose_subseteq'.
-        by apply ndot_ne_disjoint.
-      + intros.
-        apply Nat.lt_succ_r.
-        by apply Hbound.
-      + done.
-      + by iFrame.
-    - iDestruct "Hcont" as "(%&%&%&%&$&[(%&?)|(%&?)]&?)"; iModIntro; iFrame; [iLeft|iRight]; by iFrame.
-  Qed.
   
     
   Lemma con_hash_spec_test1 N f l hm γ1 γ2 γ3 γlock α n ns (v:nat):
-    {{{ con_hash_inv1 N f l hm (λ _ _, True) (λ _, True) γ1 γ2 γ3 γlock ∗ hash_tape1 α (n::ns) γ2 γ3 }}}
+    {{{ con_hash_inv1 N f l hm (λ _, True) γ1 γ2 γ3 γlock ∗ hash_tape1 α (n::ns) γ2 γ3 }}}
       f #v α
       {{{ (res:nat), RET (#res);  hash_frag1 v res γ1 γ2 ∗
                                 (hash_tape1 α ns γ2 γ3 ∗ ⌜res=n⌝ ∨
@@ -197,15 +143,12 @@ Section test.
   Proof.
     iIntros (Φ) "[#Hinv Ht] HΦ".
     iDestruct (hash_tape_in_hash_set with "[$]") as "#Hfrag".
-    iApply (con_hash_spec1 _ _ _ _ _ _ _ _ _ _ (λ res, hash_frag1 v res γ1 γ2 ∗ hash_tape1 α _ _ _)%I (λ n' ns', ⌜n=n'⌝ ∗ ⌜ns'=ns⌝ ∗ hash_frag1 v n γ1 γ2 ∗ hash_tape1 α _ _ _)%I with "[$Hinv Ht]").
-    - iIntros (??) "_ _ Htauth Hauth ".
+    iApply (con_hash_spec1 _ _ _ _ _ _ _ _ _ (λ res, hash_frag1 v res γ1 γ2 ∗ hash_tape1 α _ _ _)%I (λ n' ns', ⌜n=n'⌝ ∗ ⌜ns'=ns⌝ ∗ hash_frag1 v n γ1 γ2 ∗ hash_tape1 α _ _ _)%I with "[$Hinv Ht]").
+    - iIntros (?) "_ Hauth ".
       case_match.
       + iDestruct (hash_auth_duplicate with "[$]") as "#$"; first done. by iFrame.
-      + iDestruct (hash_tape_auth_frag_agree with "[$][$]") as "%H'".
-        iFrame. iModIntro.
-        iSplit; first done.
-        rewrite insert_id; last done.
-        iFrame.  
+      + iFrame. iModIntro.
+        iIntros. 
         iMod (hash_auth_insert with "[][$]") as "H"; first done; last first.
         * iDestruct (hash_auth_duplicate with "[$]") as "#$"; first by rewrite lookup_insert.
           iFrame. iIntros. iFrame. by done.
@@ -216,7 +159,7 @@ Section test.
   Qed.
 
   Lemma con_hash_spec_hashed_before1 N f l hm γ1 γ2 γ3 γlock α ns res (v:nat):
-    {{{ con_hash_inv1 N f l hm (λ _ _, True) (λ _, True) γ1 γ2 γ3 γlock ∗ hash_tape1 α ns γ2 γ3 ∗ hash_frag1 v res γ1 γ2 }}}
+    {{{ con_hash_inv1 N f l hm (λ _, True) γ1 γ2 γ3 γlock ∗ hash_tape1 α ns γ2 γ3 ∗ hash_frag1 v res γ1 γ2 }}}
       f #v α
       {{{ RET (#res);  hash_frag1 v res γ1 γ2 ∗
                        (hash_tape1 α ns γ2 γ3 )
@@ -224,8 +167,8 @@ Section test.
   Proof. 
     iIntros (Φ) "(#Hinv & Ht & #Hf) HΦ".
     iDestruct (hash_tape_in_hash_set with "[$]") as "#Hfrag".
-    iApply (con_hash_spec1 _ _ _ _ _ _ _ _ _ _ (λ res' , ⌜res=res'⌝ ∗ hash_frag1 v res γ1 γ2 ∗ hash_tape1 α _ _ _)%I (λ _ _, ⌜False⌝)%I with "[$Hinv Ht]").
-    - iIntros (??) "_ _ Htauth Hauth".
+    iApply (con_hash_spec1 _ _ _ _ _ _ _ _ _ (λ res' , ⌜res=res'⌝ ∗ hash_frag1 v res γ1 γ2 ∗ hash_tape1 α _ _ _)%I (λ _ _, ⌜False⌝)%I with "[$Hinv Ht]").
+    - iIntros (?) "_ Hauth".
       case_match.
       + iDestruct (hash_auth_frag_agree with "[$][$]") as "%".
         simplify_eq. iDestruct (hash_auth_duplicate with "[$]") as "#$"; first done. by iFrame.
