theories/coneris/examples/hash/con_hash_interface2.v
@@ -33,10 +33,9 @@ Class con_hash2 `{!conerisGS Σ} (val_size:nat):= Con_Hash2
   hash_set_gname':Type;
   
   (** * Predicates *)
-  con_hash_inv2 (N:namespace) (f l hm: val) (P:gmap nat nat -> gmap val (list nat) -> iProp Σ) {HP: ∀ m m', Timeless (P m m')}  (R:gmap nat nat -> iProp Σ) {HR: ∀ m, Timeless (R m )} (γ1:hash_view_gname) (γ2: hash_set_gname) (γ3:hash_tape_gname) (γ4:hash_view_gname') (γ5:hash_set_gname') (γ_lock:hash_lock_gname): iProp Σ;
+  con_hash_inv2 (N:namespace) (f l hm: val)  (R:gmap nat nat -> iProp Σ) {HR: ∀ m, Timeless (R m )} (γ1:hash_view_gname) (γ2: hash_set_gname) (γ3:hash_tape_gname) (γ4:hash_view_gname') (γ5:hash_set_gname') (γ_lock:hash_lock_gname): iProp Σ;
   (* concrete_seq_hash {L:seq_hashG Σ} (f:val) (m:gmap nat nat) : iProp Σ;  *)
   hash_tape2 (α:val) (ns:list nat) (γ2: hash_set_gname) (γ3:hash_tape_gname): iProp Σ; 
-  hash_tape_auth2 (m:gmap val (list nat)) (γ2 :hash_set_gname) (γ3:hash_tape_gname): iProp Σ;
   hash_auth2 (m:gmap nat nat) (γ:hash_view_gname) (γ2 : hash_set_gname) (γ4: hash_view_gname') (γ5:hash_set_gname'): iProp Σ; 
   hash_frag2 (v res:nat) (γ:hash_view_gname) (γ2 : hash_set_gname) (γ4:hash_view_gname'): iProp Σ;
   hash_set2 (s: nat) (γ2:hash_set_gname) (γ5:hash_set_gname'): iProp Σ;
@@ -47,8 +46,6 @@ Class con_hash2 `{!conerisGS Σ} (val_size:nat):= Con_Hash2
   (*   Timeless (concrete_seq_hash (L:=L) f m); *)
   #[global] hash_tape_timeless α ns γ2 γ3 ::
     Timeless (hash_tape2 α ns γ2 γ3 );
-  #[global] hash_tape_auth_timeless m γ2 γ3::
-    Timeless (hash_tape_auth2 m γ2 γ3);
   #[global] hash_auth_timeless m γ γ2 γ4 γ5::
     Timeless (hash_auth2 m γ γ2 γ4 γ5);
   #[global] hash_frag_timeless v res γ γ2 γ4::
@@ -57,8 +54,8 @@ Class con_hash2 `{!conerisGS Σ} (val_size:nat):= Con_Hash2
     Timeless (hash_set2 s γ2 γ5); 
   #[global] hash_set_frag_timeless s γ2 γ5 ::
     Timeless (hash_set_frag2 s γ2 γ5); 
-  #[global] con_hash_inv_persistent N f l hm γ1 γ2 γ3 P {HP: ∀ m m', Timeless (P m m')} R {HR: ∀ m, Timeless (R m )}γ4 γ5 γ_lock ::
-    Persistent (con_hash_inv2 N f l hm P R γ1 γ2 γ3 γ4 γ5 γ_lock); 
+  #[global] con_hash_inv_persistent N f l hm γ1 γ2 γ3 R {HR: ∀ m, Timeless (R m )}γ4 γ5 γ_lock ::
+    Persistent (con_hash_inv2 N f l hm R γ1 γ2 γ3 γ4 γ5 γ_lock); 
   #[global] hash_frag_persistent v res γ γ2 γ4 ::
     Persistent (hash_frag2 v res γ γ2 γ4);
   (* #[global] hash_set_frag_persistent s γ2 :: *)
@@ -83,8 +80,7 @@ Class con_hash2 `{!conerisGS Σ} (val_size:nat):= Con_Hash2
     m!!k=None -> hash_set_frag2 v γ2 γ5 -∗ hash_auth2 m γ1 γ2 γ4 γ5 ==∗ hash_auth2 (<[k:=v]> m ) γ1 γ2 γ4 γ5  ;  
   (* hash_tape_auth_exclusive m m' γ2 γ3: *)
   (*   hash_tape_auth1 m γ2 γ3 -∗ hash_tape_auth1 m' γ2 γ3 -∗ False; *)
-  hash_tape_auth_frag_agree m α ns γ2 γ3:
-    hash_tape_auth2 m γ2 γ3 -∗ hash_tape2 α ns γ2 γ3 -∗ ⌜m!!α=Some ns⌝;
+  
   (* hash_tape_auth_insert m α γ2 γ3: *)
   (*   m!!α=None -> hash_tape_auth1 m γ2 γ3 ==∗ hash_tape_auth1 (<[α:=[]]> m) γ2 γ3 ∗ hash_tape1 α [] γ2 γ3; *)
   (* hash_tape_auth_frag_update m α ns n γ2 γ3: *)
@@ -98,54 +94,39 @@ Class con_hash2 `{!conerisGS Σ} (val_size:nat):= Con_Hash2
       hash_tape2 α ns γ2 γ3 -∗ hash_tape2 α ns' γ2 γ3  -∗ False; 
 
   
-  hash_tape_presample N f l hm P {HP: ∀ m m', Timeless (P m m')} R {HR: ∀ m, Timeless (R m )} m γ_hv γ_set γ_hv' γ γ_set' γ_lock α ns s (ε εO:nonnegreal) E:
-  ↑(N.@"rand")⊆E ->
+  hash_tape_presample N f l hm R {HR: ∀ m, Timeless (R m )} γ_hv γ_set γ_hv' γ γ_set' γ_lock α ns s (ε εO:nonnegreal) E:
+  ↑(N)⊆E ->
   (INR s + εO * (val_size + 1 - INR s) <= ε * (val_size + 1))%R ->
-  con_hash_inv2 N f l hm P R γ_hv γ_set γ γ_hv' γ_set' γ_lock -∗
-    hash_tape_auth2 m γ_set γ -∗ hash_tape2 α ns γ_set γ-∗ ↯ ε -∗
+  con_hash_inv2 N f l hm R γ_hv γ_set γ γ_hv' γ_set' γ_lock -∗
+    hash_tape2 α ns γ_set γ-∗ ↯ ε -∗
     hash_set2 s γ_set γ_set'-∗
     state_update E E (∃ (n:fin(S val_size)), 
           (  hash_set2 (s+1)%nat γ_set γ_set' ∗ ↯ εO
           )∗
-          hash_tape_auth2 (<[α:=ns++[fin_to_nat n]]>m) γ_set γ ∗
           hash_tape2 α (ns++[fin_to_nat n]) γ_set γ ∗ hash_set_frag2 (fin_to_nat n) γ_set γ_set'
       );
 
-  con_hash_presample2  N f l hm P {HP: ∀ m m', Timeless (P m m')} R {HR: ∀ m, Timeless (R m )} γ_hv γ_set γ_tape γ_hv' γ_set' γ_lock Q
-    E  :
-    ↑(N.@"hash") ⊆ E ->
-    con_hash_inv2 N f l hm P R γ_hv γ_set γ_tape γ_hv' γ_set' γ_lock -∗
-    (∀ m m', P m m'  -∗
-             hash_tape_auth2 m' γ_set γ_tape -∗
-             state_update (E∖↑(N.@"hash")) (E∖↑(N.@"hash"))
-             (∃ m'', P m m'' ∗ hash_tape_auth2 m'' γ_set γ_tape ∗ Q m m' m'')
-    ) -∗
-    state_update E E (
-        ∃ m m' m'', Q m m' m''
-      ) ; 
-
-  con_hash_init2 N P {HP: ∀ m m', Timeless (P m m')} R {HR: ∀ m, Timeless (R m )}:
-    {{{ P ∅ ∅ ∗ R ∅}}}
+  con_hash_init2 N R {HR: ∀ m, Timeless (R m )}:
+    {{{ R ∅}}}
       init_hash2 #()
-      {{{ (f:val), RET f; ∃ l hm γ1 γ2 γ3 γ4 γ5 γ_lock, con_hash_inv2 N f l hm P R γ1 γ2 γ3 γ4 γ5 γ_lock ∗
+      {{{ (f:val), RET f; ∃ l hm γ1 γ2 γ3 γ4 γ5 γ_lock, con_hash_inv2 N f l hm R γ1 γ2 γ3 γ4 γ5 γ_lock ∗
                                                   hash_set2 0%nat γ2 γ5
       }}}; 
 
-  con_hash_alloc_tape2 N f l hm P {HP: ∀ m m', Timeless (P m m')} R {HR: ∀ m, Timeless (R m )} γ1 γ2 γ3 γ4 γ5 γ_lock Q:
-  {{{ con_hash_inv2 N f l hm P R γ1 γ2 γ3 γ4 γ5 γ_lock ∗
-      (∀ m m' α, P m m' -∗ ⌜α∉dom m'⌝ -∗ |={⊤∖↑N.@"hash"}=> P m (<[α:=[]]>m') ∗ Q α)
+  con_hash_alloc_tape2 N f l hm R {HR: ∀ m, Timeless (R m )} γ1 γ2 γ3 γ4 γ5 γ_lock:
+  {{{ con_hash_inv2 N f l hm R γ1 γ2 γ3 γ4 γ5 γ_lock 
   }}}
       allocate_tape2 #()
-      {{{ (α: val), RET α; hash_tape2 α [] γ2 γ3 ∗ Q α }}};  
+      {{{ (α: val), RET α; hash_tape2 α [] γ2 γ3}}};  
 
-  con_hash_spec2  N f l hm P {HP: ∀ m m', Timeless (P m m')} R {HR: ∀ m, Timeless (R m )} γ1 γ2 γ3 γ4 γ5 γ_lock Q1 Q2 α (v:nat):
-  {{{ con_hash_inv2 N f l hm P R γ1 γ2 γ3 γ4 γ5 γ_lock ∗ 
-      ( ∀ m m', R m -∗ P m m' -∗ hash_tape_auth2 m' γ2 γ3 -∗ hash_auth2 m γ1 γ2 γ4 γ5-∗ state_update (⊤∖↑N.@"hash") (⊤∖↑N.@"hash")
+  con_hash_spec2  N f l hm R {HR: ∀ m, Timeless (R m )} γ1 γ2 γ3 γ4 γ5 γ_lock Q1 Q2 α (v:nat):
+  {{{ con_hash_inv2 N f l hm R γ1 γ2 γ3 γ4 γ5 γ_lock ∗ 
+      ( ∀ m, R m -∗  hash_auth2 m γ1 γ2 γ4 γ5-∗ state_update (⊤) (⊤)
              match m!!v with
-             | Some res => R m ∗ P m m' ∗ hash_tape_auth2 m' γ2 γ3 ∗ hash_auth2 m γ1 γ2 γ4 γ5∗ Q1 res
-             | None => ∃ n ns, hash_tape2 α (n::ns) γ2 γ3 ∗ P m (<[α:=n::ns]> m') ∗ hash_tape_auth2 (<[α:=n::ns]> m') γ2 γ3 ∗
-                              (∀ m'', P m m'' -∗ hash_tape2 α (ns) γ2 γ3 -∗ ⌜m''!!α=Some (n::ns)⌝
-                                      ={⊤∖↑N.@"hash"}=∗ R (<[v:=n]> m) ∗ P (<[v:=n]> m) (<[α:=ns]> m'') ∗
+             | Some res => R m ∗ hash_auth2 m γ1 γ2 γ4 γ5∗ Q1 res
+             | None => ∃ n ns, hash_tape2 α (n::ns) γ2 γ3 ∗ 
+                              (hash_tape2 α (ns) γ2 γ3 
+                                      ={⊤}=∗ R (<[v:=n]> m) ∗ 
                                       hash_auth2 (<[v:=n]> m) γ1 γ2 γ4 γ5∗ Q2 n ns)
              end                                        
       )
@@ -162,38 +143,10 @@ Class con_hash2 `{!conerisGS Σ} (val_size:nat):= Con_Hash2
 Section test.
   Context `{conerisGS Σ, !con_hash2 val_size}.
   Definition hash_tape2' α ns γ2 γ3 γ5:= (hash_tape2 α ns γ2 γ3 ∗ [∗ list] n∈ns, hash_set_frag2 n γ2 γ5)%I.
-                                                    
-
-  Lemma con_hash_presample_test N f l hm γ1 γ2 γ3 γ4 γ5 γlock  E (ε εI εO:nonnegreal) ns α s :
-    ↑N⊆E ->
-    (INR s+ εO * (val_size + 1 - INR s) <= ε * (val_size + 1))%R ->
-    con_hash_inv2 N f l hm (λ _ _, True) (λ _, True) γ1 γ2 γ3 γ4 γ5 γlock -∗
-    hash_tape2' α ns γ2 γ3 γ5-∗
-    ↯ ε -∗
-    hash_set2 s γ2 γ5-∗
-    state_update E E (∃ (n:fin (S val_size)),
-          hash_tape2' α (ns++[fin_to_nat n]) γ2 γ3 γ5 ∗
-          ( hash_set2 (s+1)%nat γ2 γ5∗ ↯ εO
-          )
-      ).
-  Proof.
-    iIntros (Hsubset Hineq) "#Hinv [Ht Hfrag] Herr Hs".
-    iMod (con_hash_presample2 _ _ _ _ _ _ _ _ _ _ _ _
-            (λ m m' m'', (∃ n : fin (S val_size), hash_tape2 α (ns ++ [fin_to_nat n]) γ2 γ3 ∗
-                                                  ( hash_set2 (s +1)%nat γ2 γ5 ∗ ↯ εO) ∗ hash_set_frag2 (fin_to_nat n) _ _))%I with "[//][-Hfrag]") as "Hcont".
-    - by apply nclose_subseteq'.
-    - iIntros (_ ?) "_ Hauth".
-      iMod (hash_tape_presample with "[//][$][$][$][$]") as "(%&[$$]&$&$&?)".
-      + apply subseteq_difference_r; last by apply nclose_subseteq'.
-        by apply ndot_ne_disjoint.
-      + done.
-      + by iFrame. 
-    - iFrame. iDestruct "Hcont" as "(%&%&%&%&$&$&$)". by iModIntro.
-  Qed.
-  
+                 
     
   Lemma con_hash_spec_test2 N f l hm γ1 γ2 γ3 γ4 γ5 γlock α n ns (v:nat):
-    {{{ con_hash_inv2 N f l hm (λ _ _, True) (λ _, True) γ1 γ2 γ3 γ4 γ5 γlock ∗ hash_tape2' α (n::ns) γ2 γ3 γ5 }}}
+    {{{ con_hash_inv2 N f l hm (λ _, True) γ1 γ2 γ3 γ4 γ5 γlock ∗ hash_tape2' α (n::ns) γ2 γ3 γ5 }}}
       f #v α
       {{{ (res:nat), RET (#res);  hash_frag2 v res γ1 γ2 γ4 ∗
                                 (hash_tape2' α ns γ2 γ3 γ5 ∗ ⌜res=n⌝ ∨
@@ -202,32 +155,29 @@ Section test.
       }}}.
   Proof.
     iIntros (Φ) "[#Hinv [Ht Hlis]] HΦ".
-    iApply (con_hash_spec2 _ _ _ _ _ _ _ _ _ _ _ _ (λ res, hash_tape2 _ _ _ _ ∗ hash_frag2 v res γ1 γ2 γ4 ∗ [∗ list] n0 ∈ (n :: ns), hash_set_frag2 n0 γ2 γ5)%I (λ n' ns', ⌜n=n'⌝ ∗ ⌜ns=ns'⌝ ∗ hash_tape2 _ _ _ _ ∗ hash_frag2 v n γ1 γ2 γ4 ∗ [∗ list] n0 ∈ (ns), hash_set_frag2 n0 γ2 γ5)%I with "[$Hinv Ht Hlis]").
-    - iIntros (??) "_ _ Htauth Hauth".
+    iApply (con_hash_spec2 _ _ _ _ _ _ _ _ _ _ _ (λ res, hash_tape2 _ _ _ _ ∗ hash_frag2 v res γ1 γ2 γ4 ∗ [∗ list] n0 ∈ (n :: ns), hash_set_frag2 n0 γ2 γ5)%I (λ n' ns', ⌜n=n'⌝ ∗ ⌜ns=ns'⌝ ∗ hash_tape2 _ _ _ _ ∗ hash_frag2 v n γ1 γ2 γ4 ∗ [∗ list] n0 ∈ (ns), hash_set_frag2 n0 γ2 γ5)%I with "[$Hinv Ht Hlis]").
+    - iIntros (?) "_  Hauth".
       case_match.
       + iDestruct (hash_auth_duplicate with "[$]") as "#$"; first done. by iFrame.
       + iDestruct "Hlis" as "[H1 Hlis]".
-        iDestruct (hash_tape_auth_frag_agree with "[$][$]") as "%".
         iMod (hash_auth_insert with "[$][$]") as "H"; first done.
         iDestruct (hash_auth_duplicate with "[$]") as "#$"; first by rewrite lookup_insert.
-        iFrame. iModIntro. iIntros. 
-        rewrite insert_id; last done.
-        iFrame. iIntros. iFrame. done. 
+        iFrame. iModIntro. iIntros. by iFrame.
     - iNext. iIntros (res) "[(?&?&?)|(%&->&->&?&?&?)]".
       + iApply "HΦ". iFrame. iRight. iFrame.
       + iApply "HΦ". simplify_eq. iFrame. iLeft. by iFrame. 
   Qed.
 
   Lemma con_hash_spec_hashed_before2 N f l hm γ1 γ2 γ3 γ4 γ5 γlock α ns res (v:nat):
-    {{{ con_hash_inv2 N f l hm (λ _ _, True) (λ _, True) γ1 γ2 γ3 γ4 γ5 γlock ∗ hash_tape2' α ns γ2 γ3 γ5 ∗ hash_frag2 v res γ1 γ2 γ4}}}
+    {{{ con_hash_inv2 N f l hm (λ _, True) γ1 γ2 γ3 γ4 γ5 γlock ∗ hash_tape2' α ns γ2 γ3 γ5 ∗ hash_frag2 v res γ1 γ2 γ4}}}
       f #v α
       {{{ RET (#res);  hash_frag2 v res γ1 γ2 γ4 ∗
                        (hash_tape2' α ns γ2 γ3 γ5)
       }}}.
   Proof. 
     iIntros (Φ) "(#Hinv & [Ht ?] & #Hf) HΦ".
-    iApply (con_hash_spec2 _ _ _ _ _ _ _ _ _ _ _ _ (λ res' , ⌜res=res'⌝ ∗ hash_frag2 v res γ1 γ2 γ4 ∗ hash_tape2 _ _ _ _ )%I (λ _ _, ⌜False⌝)%I with "[$Hinv Ht]").
-    - iIntros (??) "_ _ Htauth Hauth".
+    iApply (con_hash_spec2 _ _ _ _ _ _ _ _ _ _ _ (λ res' , ⌜res=res'⌝ ∗ hash_frag2 v res γ1 γ2 γ4 ∗ hash_tape2 _ _ _ _ )%I (λ _ _, ⌜False⌝)%I with "[$Hinv Ht]").
+    - iIntros (?) "_ Hauth".
       case_match.
       + iDestruct (hash_auth_frag_agree with "[$][$]") as "%".
         simplify_eq. iDestruct (hash_auth_duplicate with "[$]") as "#$"; first done.
