theories/coneris/examples/hash/con_hash_interface3.v
@@ -41,10 +41,9 @@ Class con_hash3 `{!conerisGS Σ} (val_size:nat) (max_hash_size:nat) (Hpos:0<max_
   hash_token_gname:Type;
   
   (** * Predicates *)
-  con_hash_inv3 (N:namespace) (f l hm: val) (P:gmap nat nat -> gmap val (list nat) -> iProp Σ) {HP: ∀ m m', Timeless (P m m')}  (R:gmap nat nat -> iProp Σ) {HR: ∀ m, Timeless (R m )} (γ1:hash_view_gname) (γ2: hash_set_gname) (γ3:hash_tape_gname) (γ4:hash_view_gname') (γ5:hash_set_gname') (γ6: hash_token_gname) (γ_lock:hash_lock_gname): iProp Σ;
+  con_hash_inv3 (N:namespace) (f l hm: val) (R:gmap nat nat -> iProp Σ) {HR: ∀ m, Timeless (R m )} (γ1:hash_view_gname) (γ2: hash_set_gname) (γ3:hash_tape_gname) (γ4:hash_view_gname') (γ5:hash_set_gname') (γ6: hash_token_gname) (γ_lock:hash_lock_gname): iProp Σ;
   (* concrete_seq_hash {L:seq_hashG Σ} (f:val) (m:gmap nat nat) : iProp Σ;  *)
   hash_tape3 (α:val) (ns:list nat) (γ2: hash_set_gname) (γ3:hash_tape_gname): iProp Σ; 
-  hash_tape_auth3 (m:gmap val (list nat)) (γ2 :hash_set_gname) (γ3:hash_tape_gname): iProp Σ;
   hash_auth3 (m:gmap nat nat) (γ:hash_view_gname) (γ2 : hash_set_gname) (γ4: hash_view_gname') (γ5:hash_set_gname'): iProp Σ; 
   hash_frag3 (v res:nat) (γ:hash_view_gname) (γ2 : hash_set_gname) (γ4:hash_view_gname'): iProp Σ;
   hash_set3 (s: nat) (γ2:hash_set_gname) (γ5:hash_set_gname') (γ6: hash_token_gname): iProp Σ;
@@ -56,8 +55,6 @@ Class con_hash3 `{!conerisGS Σ} (val_size:nat) (max_hash_size:nat) (Hpos:0<max_
   (*   Timeless (concrete_seq_hash (L:=L) f m); *)
   #[global] hash_tape_timeless α ns γ2 γ3 ::
     Timeless (hash_tape3 α ns γ2 γ3 );
-  #[global] hash_tape_auth_timeless m γ2 γ3::
-    Timeless (hash_tape_auth3 m γ2 γ3);
   #[global] hash_auth_timeless m γ γ2 γ4 γ5::
     Timeless (hash_auth3 m γ γ2 γ4 γ5);
   #[global] hash_frag_timeless v res γ γ2 γ4::
@@ -68,8 +65,8 @@ Class con_hash3 `{!conerisGS Σ} (val_size:nat) (max_hash_size:nat) (Hpos:0<max_
     Timeless (hash_set_frag3 s γ2 γ5); 
   #[global] hash_token_timeless s γ6 ::
     Timeless (hash_token3 s γ6); 
-  #[global] con_hash_inv_persistent N f l hm γ1 γ2 γ3 P {HP: ∀ m m', Timeless (P m m')} R {HR: ∀ m, Timeless (R m )} γ4 γ5 γ6 γ_lock ::
-    Persistent (con_hash_inv3 N f l hm P R γ1 γ2 γ3 γ4 γ5 γ6 γ_lock); 
+  #[global] con_hash_inv_persistent N f l hm γ1 γ2 γ3 R {HR: ∀ m, Timeless (R m )} γ4 γ5 γ6 γ_lock ::
+    Persistent (con_hash_inv3 N f l hm R γ1 γ2 γ3 γ4 γ5 γ6 γ_lock); 
   #[global] hash_frag_persistent v res γ γ2 γ4 ::
     Persistent (hash_frag3 v res γ γ2 γ4);
   (* #[global] hash_set_frag_persistent s γ2 :: *)
@@ -94,8 +91,7 @@ Class con_hash3 `{!conerisGS Σ} (val_size:nat) (max_hash_size:nat) (Hpos:0<max_
     m!!k=None -> hash_set_frag3 v γ2 γ5 -∗ hash_auth3 m γ1 γ2 γ4 γ5 ==∗ hash_auth3 (<[k:=v]> m ) γ1 γ2 γ4 γ5  ;  
   (* hash_tape_auth_exclusive m m' γ2 γ3: *)
   (*   hash_tape_auth1 m γ2 γ3 -∗ hash_tape_auth1 m' γ2 γ3 -∗ False; *)
-  hash_tape_auth_frag_agree m α ns γ2 γ3:
-    hash_tape_auth3 m γ2 γ3 -∗ hash_tape3 α ns γ2 γ3 -∗ ⌜m!!α=Some ns⌝;
+  
   (* hash_tape_auth_insert m α γ2 γ3: *)
   (*   m!!α=None -> hash_tape_auth1 m γ2 γ3 ==∗ hash_tape_auth1 (<[α:=[]]> m) γ2 γ3 ∗ hash_tape1 α [] γ2 γ3; *)
   (* hash_tape_auth_frag_update m α ns n γ2 γ3: *)
@@ -111,57 +107,38 @@ Class con_hash3 `{!conerisGS Σ} (val_size:nat) (max_hash_size:nat) (Hpos:0<max_
   hash_token3 (n+n') γ6 ⊣⊢hash_token3 n γ6 ∗ hash_token3 n' γ6;
 
   
-  hash_tape_presample N f l hm P {HP: ∀ m m', Timeless (P m m')} R {HR: ∀ m, Timeless (R m )} m γ_hv γ_set γ_hv' γ_token γ γ_set' γ_lock α ns  E:
-  ↑(N.@"rand")⊆E ->
-  ↑(N.@"err")⊆E ->
-  con_hash_inv3 N f l hm P R γ_hv γ_set γ γ_hv' γ_set' γ_token γ_lock -∗
-  hash_tape_auth3 m γ_set γ -∗
+  hash_tape_presample N f l hm R {HR: ∀ m, Timeless (R m )} γ_hv γ_set γ_hv' γ_token γ γ_set' γ_lock α ns  E:
+  ↑(N)⊆E ->
+  con_hash_inv3 N f l hm R γ_hv γ_set γ γ_hv' γ_set' γ_token γ_lock -∗
   hash_tape3 α ns γ_set γ-∗
   ↯ (amortized_error val_size max_hash_size Hpos) -∗
   hash_token3 1 γ_token-∗
     (* hash_set3 s γ_set γ_set' γ6-∗ *)
     state_update E E (∃ (n:fin(S val_size)), 
           (* ( hash_set3 (s+1)%nat γ_set γ_set' γ6 )∗ *)
-          hash_tape_auth3 (<[α:=ns++[fin_to_nat n]]>m) γ_set γ ∗
           hash_tape3 α (ns++[fin_to_nat n]) γ_set γ ∗ hash_set_frag3 (fin_to_nat n) γ_set γ_set'
       ); 
 
-  con_hash_presample3  N f l hm P {HP: ∀ m m', Timeless (P m m')} R {HR: ∀ m, Timeless (R m )} γ_hv γ_set γ_tape γ_hv' γ_set' γ_token γ_lock Q
-    E  :
-  ↑(N.@"hash") ⊆ E ->
-  (* ↑(N.@"err") ⊆ E -> *)
-    con_hash_inv3 N f l hm P R γ_hv γ_set γ_tape γ_hv' γ_set' γ_token γ_lock -∗
-    (∀ m m', P m m'  -∗
-               (* hash_set3 s γ_set γ_set' γ_token -∗ *)
-             hash_tape_auth3 m' γ_set γ_tape -∗
-             state_update (E∖↑(N.@"hash")) (E∖↑(N.@"hash"))
-             (∃ m'' , P m m'' ∗ hash_tape_auth3 m'' γ_set γ_tape ∗  Q m m' m'' )
-    ) -∗
-    state_update E E (
-        ∃ m m' m''  , Q m m' m'' 
-      ) ; 
-
-  con_hash_init3 N P {HP: ∀ m m', Timeless (P m m')}R {HR: ∀ m, Timeless (R m )} :
-    {{{ P ∅ ∅ ∗ R ∅}}}
+  con_hash_init3 N R {HR: ∀ m, Timeless (R m )} :
+    {{{ R ∅}}}
       init_hash3 #()
-      {{{ (f:val), RET f; ∃ l hm γ1 γ2 γ3 γ4 γ5 γ_token γ_lock, con_hash_inv3 N f l hm P R γ1 γ2 γ3 γ4 γ5 γ_token γ_lock ∗  hash_token3 max_hash_size γ_token
+      {{{ (f:val), RET f; ∃ l hm γ1 γ2 γ3 γ4 γ5 γ_token γ_lock, con_hash_inv3 N f l hm R γ1 γ2 γ3 γ4 γ5 γ_token γ_lock ∗  hash_token3 max_hash_size γ_token
       }}}; 
 
-  con_hash_alloc_tape3 N f l hm P {HP: ∀ m m', Timeless (P m m')} R {HR: ∀ m, Timeless (R m )} γ1 γ2 γ3 γ4 γ5 γ_token γ_lock Q:
-  {{{ con_hash_inv3 N f l hm P R γ1 γ2 γ3 γ4 γ5 γ_token γ_lock ∗
-      (∀ m m' α, P m m' -∗ ⌜α∉dom m'⌝ -∗ |={⊤∖↑N.@"hash"}=> P m (<[α:=[]]>m') ∗ Q α)
+  con_hash_alloc_tape3 N f l hm R {HR: ∀ m, Timeless (R m )} γ1 γ2 γ3 γ4 γ5 γ_token γ_lock :
+  {{{ con_hash_inv3 N f l hm R γ1 γ2 γ3 γ4 γ5 γ_token γ_lock 
   }}}
       allocate_tape3 #()
-      {{{ (α: val), RET α; hash_tape3 α [] γ2 γ3 ∗ Q α }}};  
+      {{{ (α: val), RET α; hash_tape3 α [] γ2 γ3 }}};  
 
-  con_hash_spec3 N f l hm P {HP: ∀ m m', Timeless (P m m')} R {HR: ∀ m, Timeless (R m )} γ1 γ2 γ3 γ4 γ5 γ_token γ_lock Q1 Q2 α (v:nat):
-  {{{ con_hash_inv3 N f l hm P R γ1 γ2 γ3 γ4 γ5 γ_token γ_lock ∗ 
-      ( ∀ m m', R m -∗ P m m' -∗ hash_tape_auth3 m' γ2 γ3 -∗ hash_auth3 m γ1 γ2 γ4 γ5-∗ state_update (⊤∖↑N.@"hash") (⊤∖↑N.@"hash")
+  con_hash_spec3 N f l hm R {HR: ∀ m, Timeless (R m )} γ1 γ2 γ3 γ4 γ5 γ_token γ_lock Q1 Q2 α (v:nat):
+  {{{ con_hash_inv3 N f l hm R γ1 γ2 γ3 γ4 γ5 γ_token γ_lock ∗ 
+      ( ∀ m, R m -∗ hash_auth3 m γ1 γ2 γ4 γ5-∗ state_update (⊤) (⊤)
              match m!!v with
-             | Some res => R m ∗ P m m' ∗hash_tape_auth3 m' γ2 γ3 ∗ hash_auth3 m γ1 γ2 γ4 γ5∗ Q1 res
-             | None => ∃ n ns, hash_tape3 α (n::ns) γ2 γ3 ∗ P m (<[α:=n::ns]> m') ∗ hash_tape_auth3 (<[α:=n::ns]> m') γ2 γ3 ∗
-                              (∀ m'', P m m'' -∗  hash_tape3 α (ns) γ2 γ3 -∗ ⌜m''!!α=Some (n::ns)⌝
-                                      ={⊤∖↑N.@"hash"}=∗ R (<[v:=n]> m) ∗ P (<[v:=n]> m) (<[α:=ns]> m'') ∗
+             | Some res => R m ∗ hash_auth3 m γ1 γ2 γ4 γ5∗ Q1 res
+             | None => ∃ n ns, hash_tape3 α (n::ns) γ2 γ3 ∗ 
+                              (hash_tape3 α (ns) γ2 γ3
+                                      ={⊤}=∗ R (<[v:=n]> m) ∗
                                       hash_auth3 (<[v:=n]> m) γ1 γ2 γ4 γ5∗ Q2 n ns)
              end                                        
       )
@@ -180,36 +157,11 @@ Section test.
   Hypothesis max_hash_size_pos: (0<max_hash_size)%nat.
   Context `{conerisGS Σ, !con_hash3 val_size max_hash_size max_hash_size_pos}.
   Definition hash_tape3' α ns γ2 γ3 γ5:= (hash_tape3 α ns γ2 γ3 ∗ [∗ list] n∈ns, hash_set_frag3 n γ2 γ5)%I.
-                                                    
-
-  Lemma con_hash_presample_test N f l hm γ1 γ2 γ3 γ4 γ5 γlock γ_token E ns α :
-    ↑N⊆E ->
-    con_hash_inv3 N f l hm (λ _ _, True) (λ _, True )γ1 γ2 γ3 γ4 γ5 γ_token γlock -∗
-    hash_tape3' α ns γ2 γ3 γ5-∗
-    ↯ (amortized_error val_size max_hash_size max_hash_size_pos) -∗
-    hash_token3 1 γ_token -∗
-    state_update E E (∃ (n:fin (S val_size)),
-          hash_tape3' α (ns++[fin_to_nat n]) γ2 γ3 γ5 
-      ).
-  Proof.
-    iIntros (Hsubset) "#Hinv [Ht Hfrag] Herr Htoken".
-    iMod (con_hash_presample3 _ _ _ _ _ _ _ _ _ _ _ _ _
-            (λ m m' m'', (∃ n : fin (S val_size), hash_tape3 α (ns ++ [fin_to_nat n]) γ2 γ3 ∗
-                                                    hash_set_frag3 (fin_to_nat n) _ _))%I with "[//][-Hfrag]") as "Hcont".
-    - by apply nclose_subseteq'. 
-    - iIntros (???) "Hauth".
-      iMod (hash_tape_presample with "[//][$][$][$][$]") as "(%&$&$&$)".
-      + repeat apply subseteq_difference_r; last by apply nclose_subseteq'.
-        all: by apply ndot_ne_disjoint.
-      + apply subseteq_difference_r; last by apply nclose_subseteq'.
-        by apply ndot_ne_disjoint.
-      + done.
-    - iFrame. iDestruct "Hcont" as "(%&%&%&%&$&$)". by iModIntro.
-  Qed.
+                        
   
     
   Lemma con_hash_spec_test3 N f l hm γ1 γ2 γ3 γ4 γ5 γ_token γlock α n ns (v:nat):
-    {{{ con_hash_inv3 N f l hm (λ _ _, True) (λ _, True )γ1 γ2 γ3 γ4 γ5 γ_token  γlock ∗ hash_tape3' α (n::ns) γ2 γ3 γ5 }}}
+    {{{ con_hash_inv3 N f l hm (λ _, True )γ1 γ2 γ3 γ4 γ5 γ_token  γlock ∗ hash_tape3' α (n::ns) γ2 γ3 γ5 }}}
       f #v α
       {{{ (res:nat), RET (#res);  hash_frag3 v res γ1 γ2 γ4 ∗
                                 (hash_tape3' α ns γ2 γ3 γ5 ∗ ⌜res=n⌝ ∨
@@ -218,30 +170,29 @@ Section test.
       }}}.
   Proof.
     iIntros (Φ) "[#Hinv [Ht Hlis]] HΦ".
-    iApply (con_hash_spec3 _ _ _ _ _ _ _ _ _ _ _ _ _ (λ res, hash_frag3 v res γ1 γ2 γ4 ∗ hash_tape3 _ _ _ _ ∗ [∗ list] n0 ∈ (n :: ns), hash_set_frag3 n0 γ2 γ5 )%I (λ n' ns', ⌜n=n'⌝ ∗ ⌜ns = ns'⌝ ∗ hash_frag3 v n γ1 γ2 γ4 ∗ hash_tape3 _ _ _ _ ∗ [∗ list] n0 ∈ (ns), hash_set_frag3 n0 γ2 γ5)%I with "[$Hinv Ht Hlis]").
-    - iIntros (??) "_ _ Htauth Hauth".
+    iApply (con_hash_spec3 _ _ _ _ _ _ _ _ _ _ _ _ (λ res, hash_frag3 v res γ1 γ2 γ4 ∗ hash_tape3 _ _ _ _ ∗ [∗ list] n0 ∈ (n :: ns), hash_set_frag3 n0 γ2 γ5 )%I (λ n' ns', ⌜n=n'⌝ ∗ ⌜ns = ns'⌝ ∗ hash_frag3 v n γ1 γ2 γ4 ∗ hash_tape3 _ _ _ _ ∗ [∗ list] n0 ∈ (ns), hash_set_frag3 n0 γ2 γ5)%I with "[$Hinv Ht Hlis]").
+    - iIntros (?) "_ Hauth".
       case_match.
       + iDestruct (hash_auth_duplicate with "[$]") as "#$"; first done. by iFrame.
-      + iDestruct (hash_tape_auth_frag_agree with "[$][$]") as "%".
-        iDestruct "Hlis" as "[H1 Hlis]".
+      + iDestruct "Hlis" as "[H1 Hlis]".
         iMod (hash_auth_insert with "[$][$]") as "H"; first done.
         iDestruct (hash_auth_duplicate with "[$]") as "#$"; first by rewrite lookup_insert.
-        iFrame. iModIntro. iIntros. rewrite insert_id; last done. iFrame. iIntros. iFrame. done. 
+        iFrame. iModIntro. iIntros. by iFrame. 
     - iNext. iIntros (res) "[(?&?&?)|(%&->&->&?&?)]".
       + iApply "HΦ". iFrame. iRight. iFrame.
       + iApply "HΦ". simplify_eq. iFrame. iLeft. by iFrame.
   Qed.
 
   Lemma con_hash_spec_hashed_before3 N f l hm γ1 γ2 γ3 γ4 γ5 γtoken γlock α ns res (v:nat):
-    {{{ con_hash_inv3 N f l hm (λ _ _, True) (λ _, True) γ1 γ2 γ3 γ4 γ5 γtoken γlock ∗ hash_tape3' α ns γ2 γ3 γ5 ∗ hash_frag3 v res γ1 γ2 γ4}}}
+    {{{ con_hash_inv3 N f l hm (λ _, True) γ1 γ2 γ3 γ4 γ5 γtoken γlock ∗ hash_tape3' α ns γ2 γ3 γ5 ∗ hash_frag3 v res γ1 γ2 γ4}}}
       f #v α
       {{{ RET (#res);  hash_frag3 v res γ1 γ2 γ4 ∗
                        (hash_tape3' α ns γ2 γ3 γ5)
       }}}.
   Proof. 
     iIntros (Φ) "(#Hinv & [Ht ?] & #Hf) HΦ".
-    iApply (con_hash_spec3 _ _ _ _ _ _ _ _ _ _ _ _ _(λ res' , ⌜res=res'⌝ ∗ hash_tape3 _ _ _ _ ∗hash_frag3 v res γ1 γ2 γ4  )%I (λ _ _, ⌜False⌝)%I with "[$Hinv Ht]").
-    - iIntros (??) "_ _ Htauth Hauth".
+    iApply (con_hash_spec3 _ _ _ _ _ _ _ _ _ _ _ _ (λ res' , ⌜res=res'⌝ ∗ hash_tape3 _ _ _ _ ∗hash_frag3 v res γ1 γ2 γ4  )%I (λ _ _, ⌜False⌝)%I with "[$Hinv Ht]").
+    - iIntros (?) "_  Hauth".
       case_match.
       + iDestruct (hash_auth_frag_agree with "[$][$]") as "%".
         simplify_eq. iDestruct (hash_auth_duplicate with "[$]") as "#$"; first done.
