theories/coneris/lib/hocap_rand_alt.v
@@ -1,4 +1,6 @@
 (** * Hocap rand that generates a exclusive token as well
+      In most examples, the exclusive token is not needed since the data structure need not need to create 
+      an auth view of all the tapes. 
       Useful for building more complex data structures when we need to know all the tapes generated
       We also fix the tape bound
  *)
